check-footprints.bash
@@ -264,6 +264,11 @@ ROBINSON_PlusPlus.Meta.ChainNegPrf.dispatcher|propext,Classical.choice,Quot.soun
 ROBINSON_PlusPlus.Meta.ChainNegPrf.prf_lenc_thy|propext,Classical.choice,Quot.sound
 ROBINSON_PlusPlus.Meta.ChainNegPrf.prf_lenc_listInd|propext,Classical.choice,Quot.sound
 ROBINSON_PlusPlus.Meta.ChainNegPrf.derives_lineWF_neg_of_arity|propext,Classical.choice,Quot.sound,FOL.MetaRules.ex_elim,FOL.MetaRules.imp_intro,FOL.MetaRules.raa,ROBINSON_PlusPlus.Full.ax_induction_prim,ROBINSON_PlusPlus.Full.ax_list_induction
+ROBINSON_PlusPlus.Meta.ChainNegPrf.derives_lineWF_neg_of_concl|propext,Classical.choice,Quot.sound,FOL.MetaRules.ex_elim,FOL.MetaRules.imp_intro,FOL.MetaRules.or_elim,FOL.MetaRules.raa,ROBINSON_PlusPlus.Full.ax_induction_prim,ROBINSON_PlusPlus.Full.ax_list_induction
+ROBINSON_PlusPlus.Meta.ChainNegPrf.tc_p1|propext,Classical.choice,Quot.sound
+ROBINSON_PlusPlus.Meta.ChainNegPrf.tc_ind|propext,Classical.choice,Quot.sound
+ROBINSON_PlusPlus.Meta.ChainNegPrf.tc_listInd|propext,Classical.choice,Quot.sound
+ROBINSON_PlusPlus.Meta.ChainNegPrf.tc_qconf|propext,Classical.choice,Quot.sound
 ROBINSON_PlusPlus.Meta.ChainNegPrf.deuda_inNeg|Classical.choice,FOL.MetaRules.ex_elim,FOL.MetaRules.imp_intro,FOL.MetaRules.or_elim,FOL.MetaRules.raa,Quot.sound,ROBINSON_PlusPlus.Full.ax_induction_prim,ROBINSON_PlusPlus.Full.ax_list_induction,propext
 ROBINSON_PlusPlus.Meta.CodeWitnessPrf.SinWTs.prf_isTermCodeE1_of_In|Classical.choice,Quot.sound,propext
 ROBINSON_PlusPlus.Meta.D3BodyPrf.hA_lineWFDotAt|Classical.choice,Quot.sound,propext
